Co-authored-by: Mohan Shen <MohanShen@users.noreply.github.com>

Specs/try.lean
@@ -1,26 +1,20 @@
-import Init.Data.Basic
-import Init.Prelude
-
--- structure A where
---   (a : Nat)
---   (b : a > 0)
-
--- def c : A := { a := 1 , b := by simp }
-
--- namespace A
--- def haha (self : A) : Nat := 1
--- end A
 
 inductive TYPE_NAME
   | VARIANT1
   | VARIANT2
 
-inductive Animal
-  | Dog
-  | Cat
 
+inductive NaturalNumber
+  | Zero -- 0
+  | Succ : NaturalNumber -> NaturalNumber
 
+namespace NaturalNumber
+def add : NaturalNumber -> NaturalNumber -> NaturalNumber
+  | x, Zero => x
+  | x, Succ a => Succ (add x a)
 
-inductive Animal2
-  | Dog (weight : Nat)
-  | Cat (height : Nat) (weight : Nat)
+theorem example3 (a b : NaturalNumber) (h : Succ a = b) : Succ (Succ a) = Succ b := by
+  rw [h]
+
+  
+end NaturalNumber
