Specs.lean
@@ -4,5 +4,5 @@ import Specs.infer
 import Specs.semantics
 import Specs.vm
 
-def book_specs : Book := { chapters:=[ch_syntax, ch_infer, ch_semantics, ch_vm] }
+def book_specs : Book := { title := "Husky Language Specification", chapters:=[ch_syntax, ch_infer, ch_semantics, ch_vm] }
 def hello := "world"
