Specs/infer.lean
@@ -1,3 +1,3 @@
 import Specs.abstraction.Book
 
-def ch_infer : Chapter := { sections := [] }
+def ch_infer : Chapter := { title := "Inference", sections := [] }
