Specs/semantics.lean
@@ -1,3 +1,3 @@
 import Specs.abstraction.Book
 
-def ch_semantics : Chapter := { sections := [] }
+def ch_semantics : Chapter := { title := "Semantics", sections := [] }
